rank axioms golfing

Matroid/Constructions/RankAxioms.lean
@@ -1,6 +1,7 @@
-import Mathlib.Data.Matroid.Basic
-import Mathlib.Data.Matroid.IndepAxioms
+import Matroid.ForMathlib.Other
 import Matroid.Minor.Rank
+
+open Set
 
 /-- A matroid as defined by the (relative) rank axioms. The constructed
   `RankMatroid` can be then converted into a `Matroid` with `RankMatroid.matroid` -/
@@ -20,39 +21,46 @@ structure RankMatroid (α : Type*) where
 
   (Indep : Set α → Prop)
   (indep_maximal : ∀ ⦃X⦄, X ⊆ E → Matroid.ExistsMaximalSubsetProperty Indep X)
-  (indep_iff' : ∀ ⦃I⦄, Indep I ↔ I ⊆ E ∧ ∀ x ∈ I, relRank (I \ {x}) I > 0 )
+  (indep_iff' : ∀ ⦃I⦄, Indep I ↔ I ⊆ E ∧ ∀ x ∈ I, 0 < relRank (I \ {x}) I)
 
 namespace RankMatroid
 
-variable {α : Type*} {A B I J X : Set α} {x : α}
-
-def indepSubsets (M : RankMatroid α) (A : Set α) : Set (Set α) :=
-  {I | M.Indep I ∧ I ⊆ A}
+variable {α : Type*} {A B I J X : Set α} {x : α} {M : RankMatroid α}
 
 def Basis' (M : RankMatroid α) (I A : Set α) : Prop :=
-  I ∈ maximals (· ⊆ ·) (M.indepSubsets A)
+  I ∈ maximals (· ⊆ ·) {I | M.Indep I ∧ I ⊆ A}
 
-lemma relRank_self_eq_zero {M : RankMatroid α} : M.relRank A A = 0 := by
+@[simp] lemma relRank_self_eq_zero {M : RankMatroid α} : M.relRank A A = 0 := by
   obtain h := M.relRank_le_encard_diff A A
-  simpa only [sdiff_self, Set.bot_eq_empty, Set.encard_empty, nonpos_iff_eq_zero] using h
+  simpa only [sdiff_self, bot_eq_empty, encard_empty, nonpos_iff_eq_zero] using h
 
 lemma Indep.subset_ground {M : RankMatroid α} (h : M.Indep I) : I ⊆ M.E :=
   (M.indep_iff'.mp h).left
 
-lemma Indep.indep {M : RankMatroid α} (h : M.Indep I) : ∀ x ∈ I, M.relRank (I \ {x}) I > 0 :=
-  (M.indep_iff'.mp h).right
+lemma relRank_insert_eq_one_of_ne {M : RankMatroid α} (h : M.relRank A (insert x A) ≠ 0) :
+    M.relRank A (insert x A) = 1 := by
+  refine le_antisymm ?_ (ENat.one_le_iff_ne_zero.2 h)
+  refine (M.relRank_le_encard_diff _ _).trans ?_
+  simp only [← singleton_union, union_diff_right]
+  exact (encard_le_card diff_subset).trans_eq <| by simp
 
-lemma Indep.relRank_pos_of_sub_mem {M : RankMatroid α} (h : M.Indep I) (hx : x ∈ I) :
-    M.relRank (I \ {x}) I > 0 :=
-  h.indep x hx
+lemma relRank_diff_singleton_eq_one_of_ne {M : RankMatroid α} (h : M.relRank (A \ {x}) A ≠ 0) :
+    M.relRank (A \ {x}) A = 1 := by
+  by_cases hxA : x ∈ A
+  · simpa [h, hxA] using M.relRank_insert_eq_one_of_ne (A := A \ {x}) (x := x)
+  simp [hxA, relRank_self_eq_zero] at h
+
+lemma Indep.relRank_diff_singleton {M : RankMatroid α} (h : M.Indep I) (hx : x ∈ I) :
+    M.relRank (I \ {x}) I = 1 :=
+  relRank_diff_singleton_eq_one_of_ne ((M.indep_iff'.1 h).2 x hx).ne.symm
 
 lemma relRank_eq_diff_right {M : RankMatroid α} : M.relRank A B = M.relRank A (B \ A) := by
-  rw [M.relRank_eq_union_right A (B \ A), Set.diff_union_self, relRank_eq_union_right]
+  rw [M.relRank_eq_union_right A (B \ A), diff_union_self, relRank_eq_union_right]
 
 lemma relRank_mono_right {M : RankMatroid α} (hAB : A ⊆ B) :
     M.relRank X A ≤ M.relRank X B := by
   rw [M.relRank_eq_union_right _ A, M.relRank_eq_union_right _ B,
-    M.relRank_add_cancel Set.subset_union_right (Set.union_subset_union_left X hAB)]
+    M.relRank_add_cancel subset_union_right (union_subset_union_left X hAB)]
   simp only [self_le_add_right]
 
 lemma relRank_mono_left {M : RankMatroid α} (hAB : A ⊆ B) :
@@ -60,265 +68,129 @@ lemma relRank_mono_left {M : RankMatroid α} (hAB : A ⊆ B) :
   calc
     M.relRank B X = M.relRank B (X ∪ B) := by rw [relRank_eq_union_right]
     _ ≤ M.relRank (A ∪ B) ((A ∪ B) ∪ (A ∪ X)) := by
-      rw [Set.union_eq_right.mpr hAB, <-Set.union_assoc, Set.union_eq_left.mpr hAB, Set.union_comm]
+      rw [union_eq_right.mpr hAB, <-Set.union_assoc, union_eq_left.mpr hAB, union_comm]
     _ ≤ M.relRank ((A ∪ B) ∩ (A ∪ X)) (A ∪ X) := M.relRank_union_le_relRank_inter (A ∪ B) (A ∪ X)
-    _ = M.relRank (A ∪ (B ∩ X)) (A ∪ X) := by rw [Set.union_inter_distrib_left]
+    _ = M.relRank (A ∪ (B ∩ X)) (A ∪ X) := by rw [union_inter_distrib_left]
     _ ≤ M.relRank A (A ∪ (B ∩ X)) + M.relRank (A ∪ (B ∩ X)) (A ∪ X) := le_add_self
     _ = M.relRank A (A ∪ X) := by
       have h : (A ∪ (B ∩ X)) ⊆ (A ∪ X) :=
-        Set.union_subset_union (subset_refl A) Set.inter_subset_right
-      rw [M.relRank_add_cancel Set.subset_union_left h]
-    _ = M.relRank A X := by rw [Set.union_comm, <-relRank_eq_union_right]
+        union_subset_union (subset_refl A) inter_subset_right
+      rw [M.relRank_add_cancel subset_union_left h]
+    _ = M.relRank A X := by rw [union_comm, <-relRank_eq_union_right]
 
 lemma relRank_inter_ground {M : RankMatroid α} : M.relRank (A ∩ M.E) (B ∩ M.E) = M.relRank A B := by
   have relRank_inter_ground_self_left : ∀ ⦃A⦄, M.relRank (A ∩ M.E) A = 0 := fun A ↦ by
-    rw [relRank_eq_diff_right, Set.diff_self_inter, Set.diff_eq_compl_inter, <-nonpos_iff_eq_zero]
+    rw [relRank_eq_diff_right, diff_self_inter, diff_eq_compl_inter, <-nonpos_iff_eq_zero]
     have h : M.relRank ∅ (M.Eᶜ ∩ A) ≤ 0 := by
       rw [<-M.relRank_compl_ground_eq]
-      exact relRank_mono_right Set.inter_subset_left
+      exact relRank_mono_right inter_subset_left
     refine LE.le.trans ?_ h
-    exact relRank_mono_left <| Set.empty_subset (A ∩ M.E)
+    exact relRank_mono_left <| empty_subset (A ∩ M.E)
   symm
   calc
     M.relRank A B = M.relRank A (B ∪ A) := by rw [relRank_eq_union_right]
     _ = M.relRank (A ∩ M.E) (B ∪ A) := by
-      rw [M.relRank_add_cancel Set.inter_subset_left Set.subset_union_right,
+      rw [M.relRank_add_cancel inter_subset_left subset_union_right,
         relRank_inter_ground_self_left, zero_add]
     _ = M.relRank (A ∩ M.E) ((B ∪ A) ∩ M.E) := by
       have h : A ∩ M.E ⊆ (B ∪ A) ∩ M.E :=
-        Set.inter_subset_inter Set.subset_union_right <| subset_refl M.E
-      rw [M.relRank_add_cancel h Set.inter_subset_left, relRank_inter_ground_self_left, add_zero]
+        inter_subset_inter subset_union_right <| subset_refl M.E
+      rw [M.relRank_add_cancel h inter_subset_left, relRank_inter_ground_self_left, add_zero]
     _ = M.relRank (A ∩ M.E) (B ∩ M.E) := by
-      rw [Set.union_inter_distrib_right, <-relRank_eq_union_right]
+      rw [union_inter_distrib_right, <-relRank_eq_union_right]
 
 lemma relRank_inter_ground_left {M : RankMatroid α} (A B : Set α) :
     M.relRank (A ∩ M.E) B = M.relRank A B := by
-  rw [<-relRank_inter_ground, Set.inter_assoc, Set.inter_self, relRank_inter_ground]
+  rw [<-relRank_inter_ground, inter_assoc, inter_self, relRank_inter_ground]
 
 lemma relRank_inter_ground_right {M : RankMatroid α} (A B : Set α) :
     M.relRank A (B ∩ M.E) = M.relRank A B := by
-  rw [<-relRank_inter_ground, Set.inter_assoc, Set.inter_self, relRank_inter_ground]
+  rw [<-relRank_inter_ground, inter_assoc, inter_self, relRank_inter_ground]
 
-lemma indep_subset {M : RankMatroid α} (hJ : M.Indep J) (rIJ : I ⊆ J) : M.Indep I := by
+lemma Indep.subset {M : RankMatroid α} (hJ : M.Indep J) (rIJ : I ⊆ J) : M.Indep I := by
   refine M.indep_iff'.mpr ⟨rIJ.trans hJ.subset_ground, fun x hx ↦ ?_⟩
-  have hJ := hJ.relRank_pos_of_sub_mem (rIJ hx)
-  set A := I
-  set B := J \ {x}
-  have hAUB : J = I ∪ (J \ {x}) :=
-    (Set.union_diff_cancel' (Set.singleton_subset_iff.mpr hx) rIJ).symm
-  have hAIB : I \ {x} = I ∩ (J \ {x}) := by
-    ext y;
-    refine ⟨fun hY ↦ ?_, fun hY ↦ ?_⟩
-    · refine ⟨Set.mem_of_mem_diff hY, Set.mem_diff_singleton.mpr ?_⟩
-      refine ⟨rIJ (Set.mem_of_mem_diff hY), ?_⟩
-      have h := Set.not_mem_of_mem_diff hY
-      exact h
-    have hyB : y ∈ J \ {x} := Set.mem_of_mem_inter_right hY
-    have hynex : y ≠ x := by have := Set.not_mem_of_mem_diff hyB; exact this
-    exact ⟨Set.mem_of_mem_inter_left hY, hynex⟩
-  rw [hAUB] at hJ
-  rw [hAIB]
-  refine hJ.trans_le ?_
-  rw [Set.union_comm, Set.inter_comm]
-  exact M.relRank_union_le_relRank_inter B A
+  have e := M.relRank_union_le_relRank_inter (J \ {x}) I
+  have hJI : (J \ {x}) ∩ I = I \ {x} := by
+    rw [← inter_diff_right_comm, inter_eq_self_of_subset_right rIJ]
+  rwa [hJI, diff_union_eq_union_of_subset _ (by simpa), union_eq_self_of_subset_right rIJ,
+    hJ.relRank_diff_singleton (rIJ hx), ENat.one_le_iff_pos] at e
 
-lemma insert_indep_iff_relRank_insert_pos {M : RankMatroid α} (hI_indep : M.Indep I)
-    (hx : x ∈ M.E \ I) : M.Indep (Set.insert x I) ↔ M.relRank I (Set.insert x I) > 0 := by
-  refine ⟨fun hIx_indep ↦ ?_, fun hr ↦ ?_⟩
-  · have h := hIx_indep.indep x (Set.mem_insert x I)
-    have : Set.insert x I \ {x} = I :=
-      Set.insert_diff_self_of_not_mem (Set.not_mem_of_mem_diff hx)
-    rwa [this] at h
-  refine M.indep_iff'.mpr ?_
-  refine ⟨Set.insert_subset (Set.mem_of_mem_diff hx) hI_indep.subset_ground, ?_⟩
-  contrapose! hr
-  rcases hr with ⟨y, hy, hr⟩
-  by_cases hxy : x = y
-  · rw [hxy] at hr hx ⊢
-    have := Set.not_mem_of_mem_diff hx
-    have : Set.insert y I \ {y} = I := Set.insert_diff_self_of_not_mem this
-    rwa [this] at hr
-  have h : M.relRank (I \ {y}) (Set.insert x I) ≤ 1 := by
-    set C := (Set.insert x I)
-    set B := (Set.insert x I \ {y})
-    set A := (I \ {y})
-    have h₂ : B ⊆ C := @Set.diff_subset α (insert x I) {y}
-    have h₃ : A ⊆ B := by
-      refine Set.diff_singleton_subset_iff.mpr ?_
-      rw [Set.insert_diff_singleton]
-      exact (Set.subset_insert x I).trans (Set.subset_insert y (Set.insert x I))
-    have hrAB : M.relRank A B ≤ 1 := by
-      have h := M.relRank_le_encard_diff A B
-      rw [Set.diff_diff_right] at h
-      have h := h.trans (Set.encard_union_le (B \ I) (B ∩ {y}))
-      rw [Set.encard_eq_zero.mpr Set.diff_inter_self] at h
-      simp only [add_zero] at h
-      have : B \ I ⊆ {x} := by
-        refine Set.diff_subset_iff.mpr ?_
-        simp only [Set.union_singleton]
-        exact h₂
-      rcases Set.subset_singleton_iff_eq.mp this with h' | h'
-      · rw [h'] at h; rw [Set.encard_empty] at h; exact h.trans zero_le_one
-      rw [h'] at h; rwa [Set.encard_singleton] at h;
-    have h : M.relRank A B + M.relRank B C <= 1 := by
-      exact add_le_add hrAB hr
-    have := M.relRank_add_cancel h₃ h₂
-    rwa [<-this] at h
-  set C := (Set.insert x I)
-  set B := (I)
-  set A := (I \ {y})
-  have h' : M.relRank A C = M.relRank A B + M.relRank B C := by
-    have h₂ : B ⊆ C := Set.subset_insert x I
-    have h₃ : A ⊆ B := Set.diff_subset
-    exact M.relRank_add_cancel h₃ h₂
-  have h'' : M.relRank A B ≥ 1 := by
-    rcases Set.mem_insert_iff.mp hy with rfl | hy
-    · contradiction
-    have := hI_indep.indep y hy
-    exact ENat.one_le_iff_pos.mpr this
-  contrapose! h
-  rw [h'];
-  have h := ENat.add_one_le_of_lt h
-  simp only [zero_add] at h
-  have := add_le_add h'' h
-  rw [one_add_one_eq_two] at this
-  refine (ENat.add_one_le_iff ?refine_2.intro.intro.hm).mp this
-  exact ENat.coe_toNat_eq_self.mp rfl
+lemma indep_iff : M.Indep I ↔ ∀ x ∈ I, M.relRank (I \ {x}) I ≠ 0 := by
+  rw [M.indep_iff']
+  refine ⟨fun h x hx ↦ (h.2 x hx).ne.symm, fun h ↦ ⟨fun x hx ↦ by_contra fun hxE ↦ h x hx ?_, ?_⟩⟩
+  · rw [← relRank_inter_ground_left, ← inter_diff_right_comm, inter_diff_assoc,
+      diff_singleton_eq_self hxE, relRank_inter_ground_left, relRank_self_eq_zero]
+  exact fun x hx ↦ pos_iff_ne_zero.2 <| h x hx
 
-lemma indep_subset_maximal_iff_relRank_zero {M : RankMatroid α} (hI : I ⊆ X) (hI_indep : M.Indep I)
-    : (I ∈ (maximals (· ⊆ ·) {S | M.Indep S ∧ S ⊆ X}) ↔ M.relRank I X = 0) := by
-  refine ⟨fun hI_max ↦ ?_, fun hr ↦ ?_⟩
-  · by_cases hXI : X = I
-    · rw [hXI]; exact relRank_self_eq_zero
-    set S := {(insert x I) | x ∈ X \ I}
-    have h : ∀ A ∈ S, I ⊆ A ∧ M.relRank I A = 0 := by
-      rintro A ⟨x, hx_mem, rfl⟩
-      refine ⟨Set.subset_insert x I, ?_⟩
-      rcases (Set.mem_diff x).mpr hx_mem with ⟨hxX, hxI⟩
-      by_cases hx : x ∉ M.E
-      · rw [<-M.relRank_inter_ground, Set.insert_inter_of_not_mem hx, M.relRank_self_eq_zero]
-      simp only [not_not] at hx
-      contrapose! hI_max
-      have hI_max : M.relRank I (insert x I) > 0 := by exact pos_iff_ne_zero.mpr hI_max
-      suffices h : M.Indep (insert x I) by
-        have : (insert x I) ∈ {S | M.Indep S ∧ S ⊆ X} := ⟨h, Set.insert_subset hxX hI⟩
-        apply mem_maximals_iff.not.mpr
-        push_neg; intro; use (insert x I)
-        exact ⟨this, Set.subset_insert x I, by exact Set.ne_insert_of_not_mem I hxI⟩
-      have hxEI : x ∈ M.E \ I := by exact (Set.mem_diff x).mpr ⟨hx, hxI⟩
-      exact (insert_indep_iff_relRank_insert_pos hI_indep hxEI).mpr hI_max
-    have := M.relRank_sUnion_eq_zero h
-    have hXU : X = S.sUnion := by
-      apply Set.eq_of_subset_of_subset
-      · intro x hx; simp only [Set.mem_sUnion]
-        by_cases h : x ∈ I
-        · have hXU_ssubset := Set.ssubset_iff_subset_ne.mpr ⟨hI, Ne.symm hXI⟩
-          rcases Set.exists_of_ssubset hXU_ssubset with ⟨y, hy⟩
-          have hy := (Set.mem_diff y).mpr hy
-          set Ay := insert y I
-          have : Ay ∈ S := by use y
-          use Ay
-          exact ⟨this, (Set.subset_insert y I) h⟩
-        have hx := (Set.mem_diff x).mpr ⟨hx, h⟩
-        use insert x I
-        constructor
-        · use x
-        exact Set.mem_insert x I
-      apply Set.sUnion_subset_iff.mpr; rintro Ax ⟨x, hx_mem, rfl⟩
-      exact Set.insert_subset ((Set.mem_diff x).mpr hx_mem).left hI
-    rwa [<-hXU] at this
-  contrapose! hr
-  unfold maximals at hr;
-  simp only [Set.mem_setOf_eq, and_imp, not_and, not_forall, Classical.not_imp,
-    exists_prop, exists_and_left] at hr
-  obtain ⟨I', hI'_indep, hI', hI'_ssubset⟩ := hr hI_indep hI
-  rw [<-Set.ssubset_def] at hI'_ssubset
-  obtain ⟨x, hxI', hxI⟩ := Set.exists_of_ssubset hI'_ssubset
-  have : M.Indep (Set.insert x I) := by
-    exact indep_subset hI'_indep (Set.insert_subset hxI' hI'_ssubset.subset)
-  have hx : x ∈ M.E := hI'_indep.subset_ground hxI'
-  rw [insert_indep_iff_relRank_insert_pos hI_indep ((Set.mem_diff x).mpr ⟨hx, hxI⟩)] at this
-  have : M.relRank I X > 0 := by
-    rw [M.relRank_add_cancel (Set.subset_insert x I) (Set.insert_subset (hI' hxI') hI)]
-    exact Left.add_pos_of_pos_of_nonneg this (zero_le (M.relRank (Set.insert x I) X))
-  exact pos_iff_ne_zero.mp this
+lemma Indep.insert_indep_of_relRank_ne_zero (hI : M.Indep I) (hx : M.relRank I (insert x I) ≠ 0) :
+    M.Indep (insert x I) := by
+  suffices ∀ a ∈ I, ¬M.relRank (insert x I \ {a}) (insert x I) = 0 by
+    simpa [indep_iff, M.relRank_add_cancel diff_subset (subset_insert _ _), hx]
+  intro a haI hr
+  have hcon := M.relRank_add_cancel (show I \ {a} ⊆ I from diff_subset) (subset_insert x I)
+  have hax : x ≠ a := by rintro rfl; simp [haI] at hx
+  rw [relRank_insert_eq_one_of_ne hx, hI.relRank_diff_singleton haI, M.relRank_add_cancel
+      (show I \ {a} ⊆ insert x I \ {a} from diff_subset_diff_left (subset_insert _ _)) diff_subset,
+      hr, add_zero, ← insert_diff_singleton_comm hax,
+      relRank_insert_eq_one_of_ne (by simp [hcon])] at hcon
+  norm_num at hcon
 
-@[simps!] protected def indepMatroid (M : RankMatroid α) : IndepMatroid α where
-  E := M.E
-  Indep := M.Indep
+lemma Indep.subset_maximal_iff_relRank_zero (hI_indep : M.Indep I) (hI : I ⊆ X) :
+    (I ∈ (maximals (· ⊆ ·) {S | M.Indep S ∧ S ⊆ X}) ↔ M.relRank I X = 0) := by
+  suffices (∀ ⦃y : Set α⦄, M.Indep y → y ⊆ X → I ⊆ y → I = y) ↔ M.relRank I X = 0 by
+    simpa [mem_maximals_iff, hI_indep, hI]
+  refine ⟨fun h ↦ ?_, fun h J hJ hJX hIJ ↦ ?_⟩
+  · have h' := M.relRank_sUnion_eq_zero (S := (fun a ↦ insert a I) '' (X \ I)) (A := I)
+    simp only [mem_image, forall_exists_index, and_imp, sUnion_image] at h'
+    obtain (h_empt | hne) := (X \ I).eq_empty_or_nonempty
+    · rw [hI.antisymm (diff_eq_empty.1 h_empt), relRank_self_eq_zero]
+    simp_rw [← singleton_union, ← biUnion_distrib_union _ hne, biUnion_of_singleton,
+      singleton_union, diff_union_self, ← relRank_eq_union_right] at h'
+    apply h'
+    rintro _ x hx rfl
+    refine ⟨subset_insert _ _, by_contra fun hnez ↦ ?_⟩
+    rw [h (y := insert x I) (hI_indep.insert_indep_of_relRank_ne_zero hnez)
+      (insert_subset hx.1 hI) (subset_insert _ _)] at hx
+    simp at hx
+  obtain (rfl | hssu) := hIJ.eq_or_ssubset; rfl
+  obtain ⟨e, he⟩ := exists_of_ssubset hssu
+  rw [M.relRank_add_cancel (subset_insert e I) ((insert_subset he.1 hIJ).trans hJX),
+    add_eq_zero_iff] at h
+  have hcon := (hJ.subset (insert_subset he.1 hIJ)).relRank_diff_singleton (.inl rfl)
+  simp [he.2] at hcon
+  simp [hcon] at h
 
-  indep_empty := by
-    rw [M.indep_iff'];
-    refine ⟨Set.empty_subset M.E, fun x hx ↦ ?_⟩
-    contradiction
 
-  indep_subset := by
-    intro I J hJ rIJ
-    exact indep_subset hJ rIJ
+@[simps!] protected def matroid (M : RankMatroid α) : Matroid α :=
+  IndepMatroid.matroid <| IndepMatroid.mk
+  (E := M.E)
+  (Indep := M.Indep)
+  (indep_empty := by simp [M.indep_iff])
+  (indep_subset := fun _ _ ↦ Indep.subset)
 
-  indep_aug := by
-    have hiff : {S | M.Indep S ∧ S ⊆ M.E} = {S | M.Indep S} := by
-      ext S; constructor
-      · simp only [Set.mem_setOf_eq, and_imp]; tauto
-      simp only [Set.mem_setOf_eq]; exact fun h ↦ ⟨h, h.subset_ground⟩
+  (indep_aug := by
+    have hrw : {S | M.Indep S} = {S | M.Indep S ∧ S ⊆ M.E} :=
+      Set.ext fun I ↦ ⟨fun h ↦ ⟨h, Indep.subset_ground h⟩, fun h ↦ h.1⟩
+    intro I B hI hInmax hBmax
+    have hB : M.Indep B := hBmax.1
+    rw [hrw, hI.subset_maximal_iff_relRank_zero hI.subset_ground] at hInmax
+    rw [hrw, hB.subset_maximal_iff_relRank_zero hB.subset_ground] at hBmax
+    have hr : ¬ (M.relRank I (I ∪ B) = 0) := by
+      refine fun h0 ↦ hInmax ?_
+      rw [M.relRank_add_cancel subset_union_left (union_subset hI.subset_ground hB.subset_ground),
+        h0, zero_add]
+      simpa [hBmax] using M.relRank_mono_left (show B ⊆ I ∪ B from subset_union_right) (X := M.E)
+    rw [← hI.subset_maximal_iff_relRank_zero subset_union_left,
+      mem_maximals_iff_forall_ssubset_not_mem] at hr
+    simp only [mem_setOf_eq, hI, subset_union_left, and_self, not_and, true_and, not_forall,
+      Classical.not_imp, not_not, exists_prop, exists_and_left] at hr
+    obtain ⟨J, hIJ, hJ, hJIB⟩ := hr
+    obtain ⟨x, hxJ, hxI⟩ := exists_of_ssubset hIJ
+    refine ⟨x, ⟨?_, hxI⟩, hJ.subset <| insert_subset hxJ hIJ.subset⟩
+    obtain (h | h) := hJIB hxJ; contradiction; assumption)
 
-    intro I B hI_indep hI_nmax hB_max
-    have hB_indep := (mem_maximals_iff.mp hB_max).left
-    have hrIE : M.relRank I M.E > 0 := by
-      contrapose! hI_nmax
-      norm_num at hI_nmax
-      have := (indep_subset_maximal_iff_relRank_zero hI_indep.subset_ground hI_indep).mpr
-      rw [hiff] at this
-      exact this hI_nmax
-    have hrBE : M.relRank B M.E = 0 := by
-      have := (indep_subset_maximal_iff_relRank_zero hB_indep.subset_ground hB_indep).mp
-      rw [hiff] at this
-      exact this hB_max
-    have hrI_IUB : M.relRank I (I ∪ B) > 0 := by
-      have h₁ : I ⊆ (I ∪ B) := Set.subset_union_left
-      have h₂ : (I ∪ B) ⊆ M.E := Set.union_subset hI_indep.subset_ground hB_indep.subset_ground
-      calc
-      0 < M.relRank I M.E := by assumption
-      _ = M.relRank I (I ∪ B) + M.relRank (I ∪ B) M.E := by
-        exact M.relRank_add_cancel h₁ h₂
-      _ ≤ M.relRank I (I ∪ B) + M.relRank B M.E := by
-        apply add_le_add_left
-        exact relRank_mono_left Set.subset_union_right
-      _ = M.relRank I (I ∪ B) := by
-        rw [hrBE]
-        simp only [add_zero]
-    have hIUB_subset := (Set.union_subset hI_indep.subset_ground hB_indep.subset_ground)
-    have hI_nmax :=
-      (not_iff_not.mpr (indep_subset_maximal_iff_relRank_zero Set.subset_union_left hI_indep)).mpr
-      (Ne.symm (hrI_IUB.ne))
-    have h_maximals_nonempty :=
-      M.indep_maximal hIUB_subset I hI_indep (Set.subset_union_left)
-    rcases h_maximals_nonempty with ⟨I', ⟨hI'_indep, hI'_contains_I, hI'_in_IUB⟩, hI'_max⟩
-    by_cases hII' : I = I'
-    · rw [<-hII'] at hI'_max hI'_indep
-      simp only [Set.mem_setOf_eq, and_imp] at hI'_max
-      contrapose! hI_nmax
-      clear hI_nmax
-      rw [mem_maximals_iff]; simp only [Set.mem_setOf_eq, Set.subset_union_left, and_true, and_imp]
-      refine ⟨by assumption, ?_⟩
-      intro y hy_indep hy_in hy_within
-      have := hI'_max hy_indep hy_within hy_in hy_within
-      exact Set.Subset.antisymm hy_within (hI'_max hy_indep hy_within hy_in hy_within)
-    have : I ⊂ I' := by exact HasSubset.Subset.ssubset_of_ne hI'_contains_I hII'
-    rcases Set.exists_of_ssubset this with ⟨x, hx⟩
-    use x
-    have : x ∈ B \ I := by
-      refine (Set.mem_diff x).mpr ⟨?_, hx.right⟩
-      rcases (Set.mem_union x I B).mp (hI'_in_IUB hx.left) with h | h
-      · exfalso; exact hx.right h
-      assumption
-    refine ⟨this, ?_⟩
-    exact indep_subset hI'_indep (Set.insert_subset hx.left hI'_contains_I)
-
-  indep_maximal := fun X hX ↦ M.indep_maximal hX
-  subset_ground := fun I hI ↦ hI.subset_ground
-
-@[simps!] protected def matroid (M : RankMatroid α) : Matroid α := M.indepMatroid.matroid
+  (indep_maximal := fun X hX ↦ M.indep_maximal hX)
+  (subset_ground := fun I hI ↦ hI.subset_ground)
 
 end RankMatroid
 
@@ -328,7 +200,7 @@ variable {α : Type*} {I : Set α}
 
 lemma basis_of_maximal_extension (M : Matroid α) {I X J : Set α} (hX : X ⊆ M.E)
     (h : J ∈ maximals (· ⊆ ·) {I' | M.Indep I' ∧ I ⊆ I' ∧ I' ⊆ X}) : M.Basis J X := by
-  unfold Basis; unfold maximals at h ⊢; simp only [Set.mem_setOf_eq, and_imp] at h ⊢
+  unfold Basis; unfold maximals at h ⊢; simp only [mem_setOf_eq, and_imp] at h ⊢
   obtain ⟨⟨hJ_indep, hIJ, hJX⟩, hJ_max⟩ := h
   refine ⟨⟨⟨hJ_indep, hJX⟩, ?_⟩, hX⟩
   intro J' hJ'_indep hJ'X hJJ'
@@ -336,8 +208,8 @@ lemma basis_of_maximal_extension (M : Matroid α) {I X J : Set α} (hX : X ⊆ M
 
 lemma relRank_intro (M : Matroid α) {A B : Set α} (hA : A ⊆ B) (hB : B ⊆ M.E) :
     ∃ I J : Set α, I ⊆ J ∧ M.Basis I A ∧ M.Basis J B ∧ M.relRank A B = (J \ I).encard := by
-  obtain ⟨I, hI⟩ := M.maximality A (hA.trans hB) ∅ M.empty_indep (Set.empty_subset A)
-  unfold maximals at hI; simp only [Set.empty_subset, true_and, Set.mem_setOf_eq, and_imp] at hI
+  obtain ⟨I, hI⟩ := M.maximality A (hA.trans hB) ∅ M.empty_indep (empty_subset A)
+  unfold maximals at hI; simp only [empty_subset, true_and, mem_setOf_eq, and_imp] at hI
   have ⟨⟨hI_indep, hI_subset_A⟩, _⟩ := hI
   obtain ⟨J, hJ⟩ := M.maximality B hB I hI_indep (hI_subset_A.trans hA)
   use I; use J
@@ -345,7 +217,7 @@ lemma relRank_intro (M : Matroid α) {A B : Set α} (hA : A ⊆ B) (hB : B ⊆ M
   have hIJ : I ⊆ J := hJ.1.2.1
   have hI_basis : M.Basis I A := by
     refine @basis_of_maximal_extension α M ∅ A I (hA.trans hB) ?_
-    unfold maximals; simp only [Set.empty_subset, true_and, Set.mem_setOf_eq, and_imp]
+    unfold maximals; simp only [empty_subset, true_and, mem_setOf_eq, and_imp]
     assumption
   have hJ_basis : M.Basis J B := by
     refine M.basis_of_maximal_extension hB hJ
@@ -358,110 +230,71 @@ namespace RankMatroid
 
 variable {α : Type*} {A B I J X : Set α} {M : RankMatroid α} {x : α}
 
-lemma relRank_indeps_eq_encard_diff (M : RankMatroid α) {A B : Set α} (hA : A ⊆ B) (hB : M.Indep B)
-    : M.relRank A B = (B \ A).encard := by
-  set P := fun n ↦ ∀ (A B : Set α), A ⊆ B → M.Indep B → (B \ A).encard = n → M.relRank A B = n
-  have h_induc : ∀ n : ℕ∞, P n := by
-    intro n
-    refine (@ENat.nat_induction P n ?_ ?_ ?_)
-    · intro A B _ _ h
-      have := M.relRank_le_encard_diff A B
-      rw [h] at this; simp only [nonpos_iff_eq_zero] at this; assumption
-    · intro n hPn A B hA hB_indep h
-      have : (n.succ : ℕ∞) > 0 := by exact NeZero.pos (n.succ : ℕ∞)
-      rw [<-h] at this
-      rcases (Set.encard_pos.mp this) with ⟨x, hx⟩
-      set B' := B \ {x}
-      have hxB : x ∈ B := Set.mem_of_mem_diff hx
-      have hB'B : B' ⊆ B := by exact Set.diff_subset
-      have hAB' : A ⊆ B' := Set.subset_diff_singleton hA (Set.not_mem_of_mem_diff hx)
-      have hB'_indep : M.Indep B' := M.indep_subset hB_indep hB'B
-      have hB'dA : B' \ A = (B \ A) \ {x} := by exact Set.diff_diff_comm
-      have : (B' \ A).encard = n := by
-        rw [hB'dA]
-        rw [<-Set.encard_diff_singleton_add_one hx] at h
-        simp only [Nat.succ_eq_add_one, Nat.cast_add, Nat.cast_one] at h
-        exact WithTop.add_right_cancel (ENat.coe_toNat_eq_self.mp (refl 1)) h
-      have hrAB' : M.relRank A B' = n := hPn A B' hAB' hB'_indep this
-      have hrB'B : M.relRank B' B = 1 := by
-        have hle : M.relRank B' B <= 1 := by
-          have := M.relRank_le_encard_diff (B \ {x}) B
-          rw [Set.diff_diff_cancel_left (Set.singleton_subset_iff.mpr hxB)] at this
-          simp only [Set.encard_singleton] at this; exact this
-        have hgt : M.relRank B' B > 0 := by exact hB_indep.indep x hxB
-        refine le_antisymm_iff.mpr ⟨hle, ENat.one_le_iff_pos.mpr hgt⟩
-      rw [M.relRank_add_cancel hAB' hB'B, hrAB', hrB'B]
-      have h11: (1 : ℕ) = (1 : ℕ∞) := rfl
-      rw [<-h11, <-(ENat.coe_add n 1), Nat.succ_eq_add_one]
-    intro hP A B hB hA_indep h
-    by_contra! h_finite
-    have : ∃ n, M.relRank A B = n := exists_eq'
-    rcases this with ⟨c, hc⟩
-    simp at h
-    obtain ⟨D, hD_subset, hD_finite, hD_ncard⟩ :=
-      Set.Infinite.exists_subset_ncard_eq h (ENat.toNat c + 1)
-    have c_finite : c ≠ ⊤ := by rwa [hc] at h_finite
-    have hcc : c + 1 = ↑(ENat.toNat c + 1) := by
-      simp only [Nat.cast_add, Nat.cast_one, ENat.coe_toNat_eq_self.mpr c_finite]
-    have hD_encard : D.encard = c + 1 := by
-      have : D.encard = (D.ncard : ℕ∞) := by exact Eq.symm (Set.Finite.cast_ncard_eq hD_finite)
-      rw [this, congrArg (Nat.cast) hD_ncard, hcc]
-    clear hD_ncard hD_finite h_finite
-    let A' := A ∪ D
-    have hD_subset_B : D ⊆ B := hD_subset.trans (Set.diff_subset)
-    have hA'_subset_B : A' ⊆ B := by exact (Set.union_subset hB hD_subset_B)
-    have hA'_indep : M.Indep A' := by exact M.indep_subset hA_indep hA'_subset_B
-    have hA'A : (A' \ A).encard = ↑(ENat.toNat c + 1) := by
-      have : A ∩ D ⊆ ∅ := by
-        have : Disjoint A (B \ A) := Set.disjoint_sdiff_right
-        have : Disjoint A D := by exact Set.disjoint_of_subset (fun ⦃a⦄ a ↦ a) hD_subset this
-        exact Set.disjoint_iff.mp this
-      rw [Set.union_diff_cancel_left this, hD_encard, hcc]
-    have hrAA' : M.relRank A A' = c + 1 := by
-      rw [hP (ENat.toNat c + 1) A A' (Set.subset_union_left) hA'_indep hA'A, hcc]
-    have hbad : M.relRank A B ≥ c + 1 := by
-      rw [M.relRank_add_cancel Set.subset_union_left hA'_subset_B, hrAA']
-      simp only [ge_iff_le, self_le_add_right]
-    rw [hc] at hbad;
-    exact (lt_irrefl c) ((ENat.add_one_le_iff c_finite).mp hbad)
-  exact h_induc (B \ A).encard A B hA hB rfl
+lemma relRank_indeps_eq_encard_diff (M : RankMatroid α) {A B : Set α} (hA : A ⊆ B) (hB : M.Indep B) :
+    M.relRank A B = (B \ A).encard := by
+  classical
+  suffices aux : ∀ (D : Finset α), Disjoint A D → (D : Set α) ⊆ B → D.card ≤ M.relRank A (A ∪ D) by
+    obtain (hfin | hinf) := (B \ A).finite_or_infinite
+    · have hc : (B \ A).encard ≤ M.relRank A (A ∪ B) := by
+        simpa [disjoint_sdiff_right, diff_subset, ← hfin.encard_eq_coe_toFinset_card]
+        using aux hfin.toFinset
+      refine (M.relRank_le_encard_diff A B).antisymm ?_
+      rwa [relRank_eq_union_right, union_comm]
+    rw [hinf.encard_eq, ENat.eq_top_iff_forall_le]
+    refine fun m n hAB ↦ ⟨m, rfl, ?_⟩
+    obtain ⟨D, hDss, rfl⟩ := hinf.exists_subset_card_eq m
+    suffices (D.card : ℕ∞) ≤ n by norm_num at this; assumption
+    rw [subset_diff] at hDss
+    exact (aux D hDss.2.symm hDss.1).trans
+      ((M.relRank_mono_right (union_subset hA hDss.1)).trans_eq hAB)
+  intro D hdj hDB
+  induction' D using Finset.induction with a D haD IH; simp
+  rw [Finset.card_insert_of_not_mem haD]
+  specialize IH (hdj.mono_right (by simp)) (subset_trans (by simp) hDB)
+  rw [Nat.cast_add, Nat.cast_one, Finset.coe_insert, union_insert, ← union_singleton,
+    M.relRank_add_cancel subset_union_left subset_union_left, union_singleton,
+    relRank_insert_eq_one_of_ne]
+  · exact add_le_add_right IH 1
+  have hAuD : a ∉ A ∪ D := by
+    simp only [Finset.coe_insert, ← union_singleton, disjoint_union_right,
+      disjoint_singleton_right] at hdj; simp [haD, hdj.2]
+  nth_rw 1 [← insert_diff_self_of_not_mem hAuD, Indep.relRank_diff_singleton _ (.inl rfl)]
+  · simp
+  rw [union_comm, ←insert_union]
+  exact hB.subset (union_subset (by simpa using hDB) hA)
 
 @[simp] theorem rankMatroid_relRank_eq_matroid_relRank (M : RankMatroid α)
-    {A B : Set α} : M.relRank A B = M.matroid.relRank A B := by
+    {A B : Set α} : M.matroid.relRank A B = M.relRank A B := by
   suffices h : ∀ {A B}, A ⊆ B → B ⊆ M.E → M.relRank A B = M.matroid.relRank A B by
     set A' := A ∩ M.E
     set B' := (B ∩ M.E) ∪ A'
     rw [<-relRank_inter_ground, relRank_eq_union_right, <-M.matroid.relRank_inter_ground_left,
-        <-M.matroid.relRank_inter_ground_right, M.matroid.relRank_eq_union_right]
-    simp only [matroid_E]
-    refine h Set.subset_union_right ?_
-    rw [<-Set.union_inter_distrib_right]
-    exact Set.inter_subset_right
+        <-M.matroid.relRank_inter_ground_right, M.matroid.relRank_eq_union_right,
+        union_comm (a := B ∩ M.E), matroid_E,
+        h subset_union_left (union_subset inter_subset_right inter_subset_right),
+        union_comm]
   intro A B hA hB
   obtain ⟨I, J, hI, ⟨hI_basis_A, _⟩, ⟨hJ_basis_B, _⟩, h⟩ := M.matroid.relRank_intro hA hB
   rw [h]; clear h;
   unfold maximals at hI_basis_A hJ_basis_B;
-  simp only [matroid_Indep, Set.mem_setOf_eq, and_imp] at hI_basis_A hJ_basis_B
+  simp only [matroid_Indep, mem_setOf_eq, and_imp] at hI_basis_A hJ_basis_B
   obtain ⟨⟨hI_indep, hI_subset⟩, hI_max⟩ := hI_basis_A
   obtain ⟨⟨hJ_indep, hJ_subset⟩, hJ_max⟩ := hJ_basis_B
   rw [<-M.relRank_indeps_eq_encard_diff hI hJ_indep]
   have hIA : M.relRank I A = 0 := by
-    rw [<-indep_subset_maximal_iff_relRank_zero hI_subset hI_indep]
-    unfold maximals; simp only [Set.mem_setOf_eq, and_imp]
+    rw [<- hI_indep.subset_maximal_iff_relRank_zero hI_subset]
+    unfold maximals; simp only [mem_setOf_eq, and_imp]
     exact ⟨⟨hI_indep, hI_subset⟩, hI_max⟩
   have hJB : M.relRank J B = 0 := by
-    rw [<-indep_subset_maximal_iff_relRank_zero hJ_subset hJ_indep]
-    unfold maximals; simp only [Set.mem_setOf_eq, and_imp]
+    rw [<- hJ_indep.subset_maximal_iff_relRank_zero hJ_subset]
+    unfold maximals; simp only [mem_setOf_eq, and_imp]
     exact ⟨⟨hJ_indep, hJ_subset⟩, hJ_max⟩
   calc
-    M.relRank A B = M.relRank I A + M.relRank A B := by
-      rw [hIA]; simp only [zero_add]
-    _ = M.relRank I B := by
-      exact eq_comm.mp (M.relRank_add_cancel hI_subset hA)
-    _ = M.relRank I J + M.relRank J B := by
-      exact M.relRank_add_cancel hI hJ_subset
-    _ = M.relRank I J := by
-      rw [hJB]; simp only [add_zero]
+    M.relRank A B
+      = M.relRank I A + M.relRank A B := by rw [hIA, zero_add]
+    _ = M.relRank I B                 := by rw [M.relRank_add_cancel hI_subset hA]
+    _ = M.relRank I J + M.relRank J B := M.relRank_add_cancel hI hJ_subset
+    _ = M.relRank I J                 := by rw [hJB, add_zero]
 
 end RankMatroid
 
@@ -483,58 +316,58 @@ def ofFiniteRankAxioms {E : Set α} (hE : E.Finite) (r : Set α → ℕ)
     exact hX
   have indep_empty : Indep ∅ := by
     rw [h_indep];
-    have h := rank_le_ncard Set.finite_empty;
-    simp only [Set.encard_empty]
-    simp only [Set.ncard_empty] at h
+    have h := rank_le_ncard finite_empty;
+    simp only [encard_empty]
+    simp only [ncard_empty] at h
     exact congr_arg _ (Nat.eq_zero_of_le_zero h)
   have indep_empty_ncard : r ∅ = (∅ : Set α).ncard := by
-    have h := rank_le_ncard Set.finite_empty;
-    simp only [Set.ncard_empty] at h ⊢
+    have h := rank_le_ncard finite_empty;
+    simp only [ncard_empty] at h ⊢
     exact Nat.eq_zero_of_le_zero h
   have subset_ground : ∀ ⦃I : Set α⦄, Indep I → I ⊆ E := by
     intro I hI_indep
-    have hIE_finite : (I ∩ E).Finite := (Set.Finite.subset hE Set.inter_subset_right)
+    have hIE_finite : (I ∩ E).Finite := (Finite.subset hE inter_subset_right)
     have hIE_indep : Indep (I ∩ E) := by
       refine LE.le.antisymm ?_ ?_
       · rw [<-Set.Finite.cast_ncard_eq hIE_finite, @Nat.cast_le ℕ∞]
         exact rank_le_ncard hIE_finite
       have := submodularity (I ∩ E) (I \ E)
-      simp only [Set.inter_union_diff, rank_inter_ground (I \ E), Set.inter_assoc,
-        Set.inter_diff_self, Set.diff_inter_self, Set.inter_empty, indep_empty_ncard,
-        Set.ncard_empty, add_zero] at this
+      simp only [inter_union_diff, rank_inter_ground (I \ E), inter_assoc,
+        inter_diff_self, diff_inter_self, inter_empty, indep_empty_ncard,
+        ncard_empty, add_zero] at this
       rw [<-@Nat.cast_le ℕ∞] at this
       refine le_trans ?_ this
       rw [hI_indep]
-      exact Set.encard_mono (Set.inter_subset_left)
+      exact encard_mono (inter_subset_left)
     rw [h_indep] at hIE_indep hI_indep; rw [rank_inter_ground, hIE_indep] at hI_indep
     rw [<-Set.encard_diff_add_encard_inter I E] at hI_indep
     nth_rewrite 1 [<-zero_add (I ∩ E).encard] at hI_indep
-    exact Set.diff_eq_empty.mp (Set.encard_eq_zero.mp (WithTop.add_right_cancel
-        (Set.encard_ne_top_iff.mpr hIE_finite) hI_indep).symm)
+    exact diff_eq_empty.mp (encard_eq_zero.mp (WithTop.add_right_cancel
+        (encard_ne_top_iff.mpr hIE_finite) hI_indep).symm)
   have indep_ncard : {I : Set α} → Indep I → r I = I.ncard := by
     intro I hI
-    have hI_finite : I.Finite := Set.Finite.subset hE (subset_ground hI)
+    have hI_finite : I.Finite := Finite.subset hE (subset_ground hI)
     rw [h_indep] at hI
     rw [<-Set.Finite.cast_ncard_eq hI_finite] at hI
     refine Nat.le_antisymm (rank_le_ncard hI_finite) ?_
     rw [<-@Nat.cast_le ℕ∞, hI]
   have indep_subset : ∀ ⦃I J : Set α⦄, Indep J → I ⊆ J → Indep I := by
     intro I J hJ_indep hI
-    have hJ_finite : Set.Finite J := Set.Finite.subset hE (subset_ground hJ_indep)
-    have hI_finite : Set.Finite I := Set.Finite.subset hJ_finite hI
+    have hJ_finite : Finite J := Finite.subset hE (subset_ground hJ_indep)
+    have hI_finite : Finite I := Finite.subset hJ_finite hI
     rw [h_indep]; dsimp only
     rw [<-Set.Finite.cast_ncard_eq hI_finite]
     apply congrArg Nat.cast
     refine LE.le.antisymm (rank_le_ncard hI_finite) ?_
     have := submodularity I (J \ I)
-    rw [Set.union_diff_self, Set.inter_diff_self, indep_empty_ncard, Set.ncard_empty,
-      add_zero, Set.union_eq_self_of_subset_left hI, indep_ncard hJ_indep] at this
+    rw [union_diff_self, inter_diff_self, indep_empty_ncard, ncard_empty,
+      add_zero, union_eq_self_of_subset_left hI, indep_ncard hJ_indep] at this
     have := Nat.sub_le_of_le_add (this.trans (add_le_add (le_refl (r I))
-      (rank_le_ncard (Set.Finite.subset hJ_finite Set.diff_subset))))
-    simpa only [Set.ncard_diff hI hJ_finite,
-      Nat.sub_sub_self (Set.ncard_le_ncard hI hJ_finite)] using this
+      (rank_le_ncard (Finite.subset hJ_finite diff_subset))))
+    simpa only [ncard_diff hI hJ_finite,
+      Nat.sub_sub_self (ncard_le_ncard hI hJ_finite)] using this
   have indep_finite : ∀ ⦃I : Set α⦄, Indep I → Finite I :=
-    fun I hI ↦ Set.Finite.subset hE (subset_ground hI)
+    fun I hI ↦ Finite.subset hE (subset_ground hI)
   have indep_aug : ∀ ⦃I J : Set α⦄, Indep I → Indep J → I.ncard < J.ncard
       → ∃ e ∈ J, e ∉ I ∧ Indep (insert e I) := by
     intro I J hI_indep hJ_indep hIJ
@@ -544,38 +377,38 @@ def ofFiniteRankAxioms {E : Set α} (hE : E.Finite) (r : Set α → ℕ)
     have h : ∀ e ∈ J, e ∉ I → r (insert e I) = I.ncard := by
       intro e he he'
       have h' := this e he he'
-      rw [<-Set.Finite.cast_ncard_eq (Set.Finite.insert e hI_finite)] at h'
+      rw [<-Set.Finite.cast_ncard_eq (Finite.insert e hI_finite)] at h'
       refine Nat.le_antisymm ?_ ?_
       · have h : r (insert e I) ≠ (insert e I).ncard := by
           contrapose! h'; exact congrArg _ h'
-        have h_lt := Nat.lt_iff_le_and_ne.mpr ⟨(rank_le_ncard (Set.Finite.insert e hI_finite)), h⟩
-        rw [Set.ncard_insert_of_not_mem he' hI_finite] at h_lt
+        have h_lt := Nat.lt_iff_le_and_ne.mpr ⟨(rank_le_ncard (Finite.insert e hI_finite)), h⟩
+        rw [ncard_insert_of_not_mem he' hI_finite] at h_lt
         exact Nat.le_of_lt_succ h_lt
       rw [<-indep_ncard hI_indep]
-      exact monotonicity (Set.subset_insert e I)
+      exact monotonicity (subset_insert e I)
     have h_induc : ∀ n : ℕ, ∀ S ⊆ J \ I, S.ncard = n → r I = r (I ∪ S) := by
       intro n
       induction n with
       | zero =>
         intro S hS hS_ncard
-        have hS_finite : Finite S := Set.Finite.subset hJ_finite (hS.trans Set.diff_subset)
-        rw [(Set.ncard_eq_zero hS_finite).mp hS_ncard, Set.union_empty]
+        have hS_finite : Finite S := Finite.subset hJ_finite (hS.trans diff_subset)
+        rw [(ncard_eq_zero hS_finite).mp hS_ncard, union_empty]
       | succ n hn =>
         intro S hS hS_ncard
-        obtain ⟨y, T, hy, rfl, hT⟩ := Set.eq_insert_of_ncard_eq_succ hS_ncard
-        refine LE.le.antisymm (monotonicity (Set.subset_union_left)) ?_
-        rw [<-Set.singleton_union, Set.union_union_distrib_left]
+        obtain ⟨y, T, hy, rfl, hT⟩ := eq_insert_of_ncard_eq_succ hS_ncard
+        refine LE.le.antisymm (monotonicity (subset_union_left)) ?_
+        rw [<-Set.singleton_union, union_union_distrib_left]
         have := submodularity (I ∪ {y}) (I ∪ T)
-        nth_rw 3 [Set.union_singleton] at this
-        have hT_JI : T ⊆ J \ I := (Set.subset_insert y T).trans hS
-        have hy_JI : y ∈ J \ I := hS (Set.mem_insert y T)
-        rwa [<-hn T ((Set.subset_insert y T).trans hS) hT,
-          h y (Set.mem_of_mem_diff hy_JI) (Set.not_mem_of_mem_diff hy_JI),
-          <-Set.union_inter_distrib_left, Set.singleton_inter_eq_empty.mpr hy,
-          Set.union_empty, add_le_add_iff_right, <-indep_ncard hI_indep] at this
+        nth_rw 3 [union_singleton] at this
+        have hT_JI : T ⊆ J \ I := (subset_insert y T).trans hS
+        have hy_JI : y ∈ J \ I := hS (mem_insert y T)
+        rwa [<-hn T ((subset_insert y T).trans hS) hT,
+          h y (mem_of_mem_diff hy_JI) (not_mem_of_mem_diff hy_JI),
+          <-Set.union_inter_distrib_left, singleton_inter_eq_empty.mpr hy,
+          union_empty, add_le_add_iff_right, <-indep_ncard hI_indep] at this
     have hI_IJ := h_induc (J \ I).ncard (J \ I) subset_rfl rfl
-    simp only [Set.union_diff_self] at hI_IJ
-    have h_bad : r J ≤ r (I ∪ J) := monotonicity Set.subset_union_right
+    simp only [union_diff_self] at hI_IJ
+    have h_bad : r J ≤ r (I ∪ J) := monotonicity subset_union_right
     rw [<-hI_IJ, indep_ncard hI_indep, indep_ncard hJ_indep] at h_bad
     exact LT.lt.not_le hIJ h_bad
   exact IndepMatroid.ofFinite hE Indep indep_empty indep_subset indep_aug subset_ground
@@ -591,21 +424,21 @@ def ofFiniteRankAxioms' {E : Set α} (hE : E.Finite) (r : Set α → ℕ)
       intro n X hX
       induction n using ENat.nat_induction generalizing X with
       | h0 =>
-        rw [Set.encard_eq_zero.mp hX, rank_empty, Set.encard_empty]
+        rw [encard_eq_zero.mp hX, rank_empty, encard_empty]
         simp only [CharP.cast_eq_zero, le_refl]
       | hsuc n hn =>
         have hX_finite : Finite X := by
           have : (n.succ : ℕ∞) ≠ ⊤ := by exact ENat.coe_ne_top n.succ
-          rw [<-hX, Set.encard_ne_top_iff] at this;
+          rw [<-hX, encard_ne_top_iff] at this;
           assumption
         have h : X.ncard = n + 1 := by
           rw [<-Set.Finite.cast_ncard_eq hX_finite, Nat.succ_eq_add_one] at hX
           rwa [<-WithTop.coe_eq_coe]
-        obtain ⟨x, Y, hx, rfl, hY⟩ := Set.eq_insert_of_ncard_eq_succ h
-        have hY_finite := Set.Finite.subset hX_finite (Set.subset_insert x Y)
+        obtain ⟨x, Y, hx, rfl, hY⟩ := eq_insert_of_ncard_eq_succ h
+        have hY_finite := Finite.subset hX_finite (subset_insert x Y)
         have hY' : Y.encard = n := by
           rw [<-Set.Finite.cast_ncard_eq hY_finite, hY]
-        rw [Set.encard_insert_of_not_mem hx, <-Set.union_singleton,
+        rw [encard_insert_of_not_mem hx, <-Set.union_singleton,
           <-Set.Finite.cast_ncard_eq hY_finite, <-ENat.coe_one,
           <-ENat.coe_add Y.ncard 1, Nat.cast_le]
         have hY : r Y ≤ Y.ncard := by
@@ -619,39 +452,39 @@ def ofFiniteRankAxioms' {E : Set α} (hE : E.Finite) (r : Set α → ℕ)
     intro A B hA
     suffices h : ∀ A B, A ⊆ B → B ⊆ E → r A ≤ r B by
       rw [rank_inter_ground A, rank_inter_ground B]
-      exact h (A ∩ E) (B ∩ E) (Set.inter_subset_inter_left E hA) Set.inter_subset_right
+      exact h (A ∩ E) (B ∩ E) (inter_subset_inter_left E hA) inter_subset_right
     clear A B hA
     have h_induc : ∀ n : ℕ, ∀ {A B : Set α}, A ⊆ B → B ⊆ E → A.ncard + n = B.ncard → r A ≤ r B := by
       intro n A B hA hB
-      have hB_finite := Set.Finite.subset hE hB
-      have hA_finite := Set.Finite.subset hB_finite hA
+      have hB_finite := Finite.subset hE hB
+      have hA_finite := Finite.subset hB_finite hA
       induction n generalizing A B with
       | zero =>
         intro h; simp [add_zero] at h
-        rw [Set.eq_of_subset_of_ncard_le hA h.ge hB_finite]
+        rw [eq_of_subset_of_ncard_le hA h.ge hB_finite]
       | succ n hn =>
         intro h;
         rw [<-Set.ncard_diff_add_ncard_of_subset hA hB_finite, add_comm] at h
         simp only [add_left_inj] at h
-        obtain ⟨x, S, _, hxS, hS⟩ := Set.eq_insert_of_ncard_eq_succ h.symm
+        obtain ⟨x, S, _, hxS, hS⟩ := eq_insert_of_ncard_eq_succ h.symm
         have : B = (A ∪ S) ∪ {x} := by
-          rw [Set.union_assoc, Set.union_singleton, hxS,
-            Set.union_diff_self, Set.union_eq_self_of_subset_left hA]
-        have hAS : (A ∪ S) ⊆ B := by rw [this]; exact Set.subset_union_left
+          rw [union_assoc, union_singleton, hxS,
+            union_diff_self, union_eq_self_of_subset_left hA]
+        have hAS : (A ∪ S) ⊆ B := by rw [this]; exact subset_union_left
         have hAS_disjoint : Disjoint A S := by
-          have : S ⊆ B \ A := by rw [<-hxS]; exact Set.subset_insert x S
-          exact (Set.subset_diff.mp this).right.symm
-        have hAS_finite : (A ∪ S).Finite := Set.Finite.subset hB_finite hAS
+          have : S ⊆ B \ A := by rw [<-hxS]; exact subset_insert x S
+          exact (subset_diff.mp this).right.symm
+        have hAS_finite : (A ∪ S).Finite := Finite.subset hB_finite hAS
         have hAS_encard : A.ncard + n = (A ∪ S).ncard := by
-          rw [Set.ncard_union_eq hAS_disjoint hA_finite
-            (Set.Finite.subset hAS_finite Set.subset_union_right), add_right_inj, hS]
+          rw [ncard_union_eq hAS_disjoint hA_finite
+            (Finite.subset hAS_finite subset_union_right), add_right_inj, hS]
         rw [this]
-        exact le_trans (hn Set.subset_union_left (hAS.trans hB) hAS_finite hA_finite hAS_encard)
+        exact le_trans (hn subset_union_left (hAS.trans hB) hAS_finite hA_finite hAS_encard)
           (rank_step (A ∪ S) x).left
     intro A B hA hB
     have h_ncard : A.ncard + (B \ A).ncard = B.ncard := by
-      rw [Set.ncard_diff hA (Set.Finite.subset hE hB),
-          Nat.add_sub_cancel' (Set.ncard_le_ncard hA (Set.Finite.subset hE hB))]
+      rw [ncard_diff hA (Finite.subset hE hB),
+          Nat.add_sub_cancel' (ncard_le_ncard hA (Finite.subset hE hB))]
     exact h_induc (B \ A).ncard hA hB h_ncard
   exact IndepMatroid.ofFiniteRankAxioms hE r
     rank_le_ncard monotonicity submodularity rank_inter_ground
